src/Narcissus/Examples/NetworkStack/EthernetHeader.v
@@ -1,48 +1,43 @@
 Require Import
         Coq.Strings.String
-        Coq.Vectors.Vector.
+        Coq.Vectors.Vector
+        Coq.omega.Omega.
 
 Require Import
+        Fiat.Common.SumType
         Fiat.Common.EnumType
         Fiat.Common.BoundedLookup
         Fiat.Common.ilist
-        Fiat.Common.Tactics.CacheStringConstant
         Fiat.Computation
         Fiat.QueryStructure.Specification.Representation.Notations
         Fiat.QueryStructure.Specification.Representation.Heading
         Fiat.QueryStructure.Specification.Representation.Tuple
-        Fiat.Narcissus.BinLib.Core
+        Fiat.Narcissus.BinLib
         Fiat.Narcissus.Common.Specs
         Fiat.Narcissus.Common.WordFacts
+        Fiat.Narcissus.Common.ComposeCheckSum
         Fiat.Narcissus.Common.ComposeIf
         Fiat.Narcissus.Common.ComposeOpt
-        Fiat.Narcissus.Automation.Solver
-        Fiat.Narcissus.Formats.FixListOpt
+        Fiat.Narcissus.Formats
+        Fiat.Narcissus.BaseFormats
         Fiat.Narcissus.Stores.EmptyStore
-        Fiat.Narcissus.Formats.WordOpt
-        Fiat.Narcissus.Formats.NatOpt
-        Fiat.Narcissus.Formats.Vector
-        Fiat.Narcissus.Formats.EnumOpt
-        Fiat.Narcissus.Formats.SumTypeOpt.
+        Fiat.Narcissus.Automation.Solver
+        Fiat.Narcissus.Automation.AlignedAutomation.
 
 Require Import Bedrock.Word.
 
 Import Vectors.VectorDef.VectorNotations.
-Open Scope string_scope.
-Open Scope Tuple_scope.
-
+Open Scope format_scope.
 Opaque pow2. (* Don't want to be evaluating this. *)
 Opaque natToWord. (* Or this. *)
-
-Definition monoid : Monoid ByteString := ByteStringQueueMonoid.
 
 (* Start Example Derivation. *)
 Section EthernetPacketDecoder.
 
-  Definition EthernetHeader :=
-    @Tuple <"Destination" :: Vector.t char 6,
-    "Source" :: Vector.t char 6,
-    "Type" :: EnumType ["ARP"; "IP"; "RARP"]>.
+  Record EthernetHeader :=
+    {Destination : Vector.t (word 8) 6;
+     Source : Vector.t (word 8) 6;
+     EthType : EnumType ["ARP"; "IP"; "RARP"]}.
 
   Definition EtherTypeCodes : Vector.t (word 16) 3 :=
     [WO~0~0~0~0~1~0~0~0~0~0~0~0~0~1~1~0;
@@ -54,19 +49,38 @@ Section EthernetPacketDecoder.
   (* which is a parameter to the formatr and decoder. *)
   Variable packet_len_OK : lt packet_len 1501.
 
-  Definition format_EthernetHeader_Spec (eth : EthernetHeader) :=
-    format_Vector format_word eth!"Destination"
-                       ThenC (format_Vector format_word eth!"Source")
-                       ThenC Either
-                       format_nat 16 packet_len
-                       ThenC format_word (WO~0~1~0~1~0~1~0~1)
-                       ThenC format_word (WO~0~1~0~1~0~1~0~1)
-                       ThenC format_word (WO~1~1~0~0~0~0~0~0)
-                       ThenC format_word (wzero 24)
-                       ThenC format_enum EtherTypeCodes eth!"Type"
-                       DoneC
-                       Or format_enum EtherTypeCodes eth!"Type"
-                       DoneC.
+  Definition EthernetHeader_Format
+    : FormatM EthernetHeader ByteString :=
+    format_Vector format_word ◦ Destination
+   ++ format_Vector format_word ◦ Source
+   ++ Either
+   format_nat 16 ◦ (fun _ => packet_len)
+   ++ format_word ◦ (fun _ => WO~0~1~0~1~0~1~0~1)
+   ++ format_word ◦ (fun _ => WO~0~1~0~1~0~1~0~1)
+   ++ format_word ◦ (fun _ => WO~1~1~0~0~0~0~0~0)
+   ++ format_word ◦ (fun _ => wzero 24)
+   ++ format_enum EtherTypeCodes ◦ EthType
+   Or format_enum EtherTypeCodes ◦ EthType.
+
+  Definition EthernetHeader_encoder :
+    CorrectAlignedEncoderFor EthernetHeader_Format.
+  Proof.
+    start_synthesizing_encoder.
+    (decompose_aligned_encoder; eauto).
+    (decompose_aligned_encoder; eauto).
+    eapply CorrectAlignedEncoderEither_E; intros.
+    repeat align_encoder_step.
+    repeat align_encoder_step; eauto.
+    repeat align_encoder_step; eauto.
+    Grab Existential Variables.
+    eauto.
+    eauto.
+  Defined.
+
+  (* Step Two: Extract the encoder function, and have it start encoding
+     at the start of the provided ByteString [v]. *)
+  Definition EthernetHeader_encoder_impl r {sz} v :=
+    Eval simpl in (projT1 EthernetHeader_encoder sz v 0 r tt).
 
   Definition ethernet_Header_OK (e : EthernetHeader) := True.
 
@@ -76,24 +90,37 @@ Section EthernetPacketDecoder.
     | _ => false
     end.
 
+  Opaque natToWord.
+
   Lemma v1042_OKT
     : forall (data : EthernetHeader) (bin : ByteString) (env xenv : CacheFormat) (ext : ByteString),
-      (format_nat 16 packet_len
-                       ThenC format_word WO~0~1~0~1~0~1~0~1
-                       ThenC format_word WO~0~1~0~1~0~1~0~1
-                       ThenC format_word WO~1~1~0~0~0~0~0~0
-                       ThenC format_word (wzero 24) ThenC format_enum EtherTypeCodes data!"Type" DoneC) env
-                                                                                                                  ↝ (bin, xenv) -> v1042_test (mappend bin ext) = true.
+      ((format_nat 16 packet_len
+   ThenC (fun ctx'1 : CacheFormat =>
+          (format_word WO~0~1~0~1~0~1~0~1
+           ThenC (fun ctx'2 : CacheFormat =>
+                  (format_word WO~0~1~0~1~0~1~0~1
+                   ThenC (fun ctx'3 : CacheFormat =>
+                          (format_word WO~1~1~0~0~0~0~0~0
+                           ThenC (fun ctx'4 : CacheFormat =>
+                                  (format_word (wzero 24)
+                                   ThenC (fun ctx'5 : CacheFormat =>
+                                          (format_enum EtherTypeCodes (EthType data) DoneC) ctx'5)) ctx'4)) ctx'3))
+                    ctx'2)) ctx'1)) env)
+                                            ↝ (bin, xenv) -> v1042_test (mappend bin ext) = true.
   Proof.
     intros.
-    unfold compose at 1 in H; unfold Bind2 in H;
-      computes_to_inv; destruct v; destruct v0; simpl in *;
+    unfold sequence_Format, compose at 1, Bind2 in H;
+      computes_to_inv; destruct v; destruct v0.
         injections.
-    unfold format_nat, format_word in H; computes_to_inv.
-    pose proof (f_equal fst H) as H''; simpl in H''; rewrite <- H''.
     pose proof mappend_assoc as H'''; simpl in H'''; rewrite <- H'''.
     unfold v1042_test.
-    pose monoid_get_encode_word' as H''''; rewrite H''''; find_if_inside; eauto.
+    pose proof (monoid_get_encode_word' 16 (natToWord 16 packet_len)) as H''''.
+    unfold format_nat, format_word in H; computes_to_inv.
+    apply (f_equal fst) in H; simpl in H.
+    rewrite <- H.
+    simpl mappend in *.
+    rewrite H''''.
+    find_if_inside; eauto.
     destruct n.
     eapply natToWord_wlt; eauto; try reflexivity.
     etransitivity.
@@ -106,22 +133,19 @@ Section EthernetPacketDecoder.
 
   Lemma v1042_OKE
     : forall (data : EthernetHeader) (bin : ByteString) (env xenv : CacheFormat) (ext : ByteString),
-      (format_enum EtherTypeCodes data!"Type" DoneC) env ↝ (bin, xenv)
+      (format_enum EtherTypeCodes (EthType data) DoneC) env ↝ (bin, xenv)
       -> v1042_test (mappend bin ext) = false.
   Proof.
-    intros; unfold compose at 1 in H; unfold Bind2 in H;
-      computes_to_inv; destruct v; destruct v0; simpl in *;
-        injections.
-    unfold format_enum, format_word in H; computes_to_inv.
-    pose proof (f_equal fst H) as H'; unfold fst in H'; rewrite <- H'.
-    pose proof mappend_assoc as H''; simpl in H''; rewrite <- H''.
+    intros.
+    unfold compose, Bind2, format_enum, format_word in H; computes_to_inv; subst.
+    pose proof (f_equal fst H'') as H'; unfold fst in H'; rewrite <- H'.
     unfold v1042_test.
+    rewrite mempty_right.
     pose monoid_get_encode_word' as H'''; rewrite H'''; find_if_inside; eauto.
     revert w; clear.
     match goal with
       |- context [Vector.nth (m := ?n) ?w ?idx] => remember idx; clear
     end.
-    Local Transparent natToWord.
     eapply forall_Vector_P; repeat econstructor;
       unfold wlt; compute; intros; discriminate.
   Qed.
@@ -140,14 +164,98 @@ Section EthernetPacketDecoder.
 
   Hint Resolve valid_packet_len_OK_good_Len : data_inv_hints.
 
-  Definition EthernetHeader_decoder
-    : CorrectDecoderFor ethernet_Header_OK format_EthernetHeader_Spec.
-  Proof.
-    synthesize_decoder.
-  Defined.
+  Definition aligned_v1042_test
+        {sz : nat}
+        (v : t Core.char sz)
+        (idx : nat)
+    : bool :=
+    match nth_opt v idx, nth_opt v (S idx) with
+    | Some w1, Some w2 =>
+      if wlt_dec (combine w2 w1) (natToWord 16 1501) then true else false
+    | _, _ => false
+    end.
 
-  Definition frame_decoder := Eval simpl in proj1_sig EthernetHeader_decoder.
+  Lemma aligned_v1042_test_OK {sz}
+    : forall (v : t Core.char sz),
+      v1042_test (build_aligned_ByteString v) =
+      aligned_v1042_test v 0.
+  Proof.
+    destruct v.
+    reflexivity.
+    destruct v.
+    reflexivity.
+    unfold v1042_test.
+    replace (monoid_get_word 16 (build_aligned_ByteString (h :: h0 :: v)))
+      with
+        (Some (combine h0 h)).
+    reflexivity.
+    replace (build_aligned_ByteString (h :: h0 :: v))
+      with (mappend (build_aligned_ByteString (h :: h0 :: Vector.nil _)) (build_aligned_ByteString v)).
+    rewrite <- (monoid_get_encode_word' _ (combine h0 h) (build_aligned_ByteString v)).
+    f_equal.
+    f_equal.
+    simpl.
+    unfold Core.char in *.
+    shatter_word h.
+    shatter_word h0.
+    simpl.
+    rewrite build_aligned_ByteString_cons; simpl.
+    unfold ByteString_enqueue_ByteString; simpl.
+    unfold ByteString_enqueue_char.
+    simpl.
+    repeat f_equal.
+    unfold build_aligned_ByteString; simpl.
+    erewrite (ByteString_enqueue_simpl x6); simpl.
+    erewrite (ByteString_enqueue_simpl x5); simpl.
+    erewrite (ByteString_enqueue_simpl x4); simpl.
+    erewrite (ByteString_enqueue_simpl x3); simpl.
+    erewrite (ByteString_enqueue_simpl x2); simpl.
+    erewrite (ByteString_enqueue_simpl x1); simpl.
+    erewrite (ByteString_enqueue_simpl x0); simpl.
+    unfold ByteString_enqueue; simpl.
+    f_equal.
+    eapply Core.le_uniqueness_proof.
+    simpl.
+    rewrite <- build_aligned_ByteString_append.
+    reflexivity.
+    Grab Existential Variables.
+    simpl; omega.
+    simpl; omega.
+    simpl; omega.
+    simpl; omega.
+    simpl; omega.
+    simpl; omega.
+    simpl; omega.
+  Qed.
+
+  Definition EthernetHeader_decoder
+    : CorrectAlignedDecoderFor ethernet_Header_OK EthernetHeader_Format.
+  Proof.
+  (* We have to use an extra lemma at the start, because of the 'exotic'
+     IP Checksum. *)
+  (* Once that's done, the normal automation works just fine :) *)
+  start_synthesizing_decoder.
+  match goal with
+  | |- CorrectDecoder ?monoid _ _ _ _ _ => normalize_compose monoid
+  end.
+  repeat decode_step ltac:(idtac).
+  cbv beta; synthesize_cache_invariant.
+  (* Perform algebraic simplification of the decoder implementation. *)
+  cbv beta; unfold decode_nat; optimize_decoder_impl.
+  cbv beta; align_decoders.
+  eapply @AlignedDecode_ifb_dep.
+  intros; rewrite aligned_v1042_test_OK; higher_order_reflexivity.
+  simpl; intros; pattern sz, v; eapply Vector.caseS; reflexivity.
+  repeat align_decoders_step.
+  repeat align_decoders_step.
+Defined.
+
+(* Step Four: Extract the decoder function, and have /it/ start decoding
+   at the start of the provided ByteString [v]. *)
+
+Definition Ethernet_decoder_impl {sz} v :=
+  Eval simpl in (projT1 EthernetHeader_decoder sz v 0 ()).
 
 End EthernetPacketDecoder.
 
-Print frame_decoder.
+Print Ethernet_decoder_impl.
